ironfleet/src/Dafny/Distributed/Protocol/RSL/PerformanceProof/PerformanceProof.i.dfy
@@ -21,6 +21,8 @@ predicate RslAssumption(s:TimestampedRslState)
   // TODO: Remove this assumption
   && (var nextStep := s.t_environment.nextStep; nextStep.LEnvStepHostIos? ==>
   (forall io :: io in nextStep.ios && io.LIoOpReceive? ==> !io.r.msg.v.RslMessage_Heartbeat?))
+  && ViewAlwaysZero(s)
+  && SelfDelivery <= D
 }
 
 predicate RslConsistency(s:TimestampedRslState)
@@ -33,16 +35,19 @@ predicate ViewAlwaysZero(s:TimestampedRslState)
 {
   && (forall idx:: 0 <= idx < |s.t_replicas|
     ==>
-    s.t_replicas[idx].v.replica.proposer.election_state.current_view.proposer_id == 0
+    s.t_replicas[idx].v.replica.proposer.election_state.current_view == Ballot(1, 0)
     )
 }
 
 predicate AlwaysInvariant(s:TimestampedRslState)
 {
-  && ViewAlwaysZero(s)
+  && (forall pkt :: pkt in s.undeliveredPackets ==>
+    pkt in s.t_environment.sentPackets
+    && pkt.src in s.constants.config.replica_ids
+    && pkt.dst in s.constants.config.replica_ids)
 }
 
-predicate LSchedulerTimeBound(tls:TimestampedLScheduler)
+predicate LSchedulerLagTimeBound(tls:TimestampedLScheduler)
 {
   0 <= tls.v.nextActionIndex <= 9
   && TimeLe(tls.ts, tls.dts + TimeActionRange(tls.v.nextActionIndex))
@@ -51,19 +56,23 @@ predicate LSchedulerTimeBound(tls:TimestampedLScheduler)
 predicate InitInvariant(s:TimestampedRslState)
   requires RslConsistency(s)
 {
+  && AlwaysInvariant(s)
+
   && (0 < |s.t_replicas|
     ==>
     var r := s.t_replicas[0].v.replica.proposer;
     (if s.t_replicas[0].v.nextActionIndex == 0 then
-      TimeEq(s.t_replicas[0].ts, TimeZero())
+      && TimeEq(s.t_replicas[0].ts, TimeZero())
+      && TimeLe(s.t_replicas[0].dts, TimeZero())
     else
       && s.t_replicas[0].v.nextActionIndex == 1
       && TimeLe(s.t_replicas[0].ts, Timeout() + ProcessPacket)
+      && TimeEq(s.t_replicas[0].dts, Timeout())
     )
   )
 
   && (forall idx :: 0 < idx < |s.t_replicas|
-  ==> LSchedulerTimeBound(s.t_replicas[idx])
+  ==> LSchedulerLagTimeBound(s.t_replicas[idx])
   )
 
   && (0 < |s.t_replicas| ==>
@@ -71,6 +80,7 @@ predicate InitInvariant(s:TimestampedRslState)
     && p.current_state == 0
     && p.election_state.current_view == Ballot(1, 0)
     && p.max_ballot_i_sent_1a == Ballot(0, 0)
+    && |p.received_1b_packets| == 0
   )
 
   && (forall idx :: 0 <= idx < |s.t_replicas|
@@ -85,69 +95,146 @@ predicate InitInvariant(s:TimestampedRslState)
   )
 }
 
-predicate No1aToDst(undeliveredPackets:multiset<TimestampedLPacket<EndPoint, RslMessage>>, dst:NodeIdentity)
+predicate No1aToDst(undeliveredPackets:UndeliveredPackets, dst:NodeIdentity)
 {
   && (forall pkt :: pkt in undeliveredPackets
     && pkt.msg.v.RslMessage_1a?
     ==> pkt.dst != dst)
 }
 
-predicate Phase1Invariant(s:TimestampedRslState)
-  requires RslConsistency(s)
+//predicate TriggerPacket(pkt:TimestampedRslPacket)
+//{
+  //true
+//}
+//
+//predicate TriggerIdx(idx:int)
+//{
+  //true
+//}
+
+predicate Phase1GenericUndeliveredPacketsInvariant(undeliveredPackets:UndeliveredPackets, constants:LConstants)
 {
-  && (forall idx :: 0 <= idx < |s.t_replicas|
-    ==>
-  && s.t_replicas[idx].v.replica.executor.next_op_to_execute == OutstandingOpUnknown()
-  && s.t_replicas[idx].v.replica.learner.unexecuted_learner_state == map[]
-  )
-
-  && (forall idx :: 0 < idx < |s.t_replicas|
-  ==>
-  && s.t_replicas[idx].v.replica.proposer.current_state == 0
-  )
-
-  && (0 < |s.t_replicas| ==>
-    && TimeLe(s.t_replicas[0].ts, TimeBound1aSent())
-  )
-  && (0 < |s.t_replicas| ==>
-    && s.t_replicas[0].v.replica.proposer.current_state == 1
-  )
-
-  && (forall pkt :: pkt in s.undeliveredPackets
+  && (forall pkt :: && pkt in undeliveredPackets
   ==>
    || pkt.msg.v.RslMessage_Heartbeat?
    || pkt.msg.v.RslMessage_1a?
    || pkt.msg.v.RslMessage_1b?
   )
 
-  && (forall pkt :: pkt in s.undeliveredPackets
+  && (forall pkt :: && pkt in undeliveredPackets
   && pkt.msg.v.RslMessage_1b?
-  ==> pkt.dst == s.constants.config.replica_ids[0]
-  // && TimeLe(pkt.msg.ts, TimeBound1bSent())
+  && 0 < |constants.config.replica_ids|
+  ==> pkt.dst == constants.config.replica_ids[0]
+  && TimeLe(pkt.msg.ts, TimeBound1bDelivery())
   )
 
-  && (forall pkt :: pkt in s.undeliveredPackets
+  && (forall pkt :: && pkt in undeliveredPackets
       && pkt.msg.v.RslMessage_1a?
-   ==> TimeLe(pkt.msg.ts, TimeBound1aSent())
+      && 0 < |constants.config.replica_ids|
+   ==> TimeLe(pkt.msg.ts, TimeBound1aDelivery())
       && pkt.msg.v.bal_1a == Ballot(1, 0)
-      && pkt.src == s.constants.config.replica_ids[0]
+      && pkt.src == constants.config.replica_ids[0]
 
-      && (var undeliveredPackets' := s.undeliveredPackets - multiset({pkt});
+      && (var undeliveredPackets' := undeliveredPackets - {pkt};
           No1aToDst(undeliveredPackets', pkt.dst)
         )
   )
+}
 
-  && (forall idx :: 0 < idx < |s.t_replicas|
+predicate Phase1GenericInvariant(s:TimestampedRslState)
+  requires RslConsistency(s)
+{
+  && AlwaysInvariant(s)
+  && Phase1GenericUndeliveredPacketsInvariant(s.undeliveredPackets, s.constants)
+
+  && (forall idx :: && 0 <= idx < |s.t_replicas|
+    ==>
+  && s.t_replicas[idx].v.replica.executor.next_op_to_execute == OutstandingOpUnknown()
+  && s.t_replicas[idx].v.replica.learner.unexecuted_learner_state == map[]
+  )
+
+  && (forall idx :: && 0 < idx < |s.t_replicas|
+  ==>
+  && s.t_replicas[idx].v.replica.proposer.current_state == 0
+  )
+
+  && (0 < |s.t_replicas| ==>
+    && s.t_replicas[0].v.replica.proposer.current_state == 1
+    && s.t_replicas[0].v.replica.proposer.max_ballot_i_sent_1a == s.t_replicas[0].v.replica.proposer.election_state.current_view
+  )
+
+  && (0 < |s.t_replicas|
+  ==> forall pkt :: pkt in s.undeliveredPackets
+  ==> UntagLPacket(pkt) !in s.t_replicas[0].v.replica.proposer.received_1b_packets
+  )
+
+  && (forall idx :: && 0 < idx < |s.t_replicas|
   ==>
   if s.t_replicas[idx].v.replica.acceptor.max_bal == Ballot(0, 0) then
-    LSchedulerTimeBound(s.t_replicas[idx])
+    LSchedulerLagTimeBound(s.t_replicas[idx])
   else
-    (forall pkt :: pkt in s.undeliveredPackets
-    && pkt.msg.v.RslMessage_1a?
-    ==> pkt.dst != s.constants.config.replica_ids[idx]
-    // (&& s.t_replicas[idx].v.replica.acceptor.max_bal == s.t_replicas[0].v.replica.proposer.max_ballot_i_sent_1a
-    // && true // TimeLe(s.t_replicas[idx].ts, TimeBound1aReceived())
+    (
+    No1aToDst(s.undeliveredPackets, s.constants.config.replica_ids[idx])
     )
+  )
+}
+
+predicate UnpreparedLeaderPhase1TimeBound(leader:TimestampedLScheduler, undeliveredPackets:UndeliveredPackets, leader_id:NodeIdentity, pkt:TimestampedRslPacket)
+{
+  && leader.v.replica.proposer.current_state == 1
+    && leader.v.replica.acceptor.max_bal == Ballot(0, 0)
+    && leader.v.replica.proposer.max_ballot_i_sent_1a == Ballot(1, 0)
+    && LSchedulerLagTimeBound(leader)
+    && pkt in undeliveredPackets
+    && pkt.msg.v == RslMessage_1a(leader.v.replica.proposer.max_ballot_i_sent_1a)
+    && pkt.src == pkt.dst == leader_id
+    && TimeLe(pkt.msg.ts, TimeBound1aSelfDelivery())
+    && No1aToDst(undeliveredPackets - {pkt}, leader_id)
+    && |leader.v.replica.proposer.received_1b_packets| == 0
+}
+
+predicate PreparedLeaderPhase1TimeBound(leader:TimestampedLScheduler, undeliveredPackets:UndeliveredPackets, leader_id:NodeIdentity)
+{
+  && leader.v.replica.proposer.current_state == 1
+    && leader.v.replica.acceptor.max_bal == leader.v.replica.proposer.max_ballot_i_sent_1a
+    && No1aToDst(undeliveredPackets, leader_id)
+    && 0 <= leader.v.nextActionIndex < 10
+    && (var ell := |leader.v.replica.proposer.received_1b_packets|;
+        TimeLe(leader.ts, TimeBoundPhase1Leader(leader.dts, ell, leader.v.nextActionIndex))
+    )
+}
+
+predicate Phase1UnpreparedLeaderInvariant(s:TimestampedRslState, leader_1a_pkt:TimestampedRslPacket)
+  requires RslConsistency(s)
+{
+  && (0 < |s.t_replicas| ==>
+    && UnpreparedLeaderPhase1TimeBound(s.t_replicas[0], s.undeliveredPackets, s.constants.config.replica_ids[0], leader_1a_pkt)
+  )
+  && (forall pkt :: && pkt in s.undeliveredPackets && pkt.msg.v.RslMessage_1b?
+  ==> pkt.src in s.constants.config.replica_ids[1..]
+  && TimeBound1aSelfDelivery() < pkt.msg.ts
+  )
+
+  && Phase1GenericInvariant(s)
+}
+
+predicate Phase1PreparedLeaderInvariant(s:TimestampedRslState)
+  requires RslConsistency(s)
+{
+  && (0 < |s.t_replicas| ==>
+    && PreparedLeaderPhase1TimeBound(s.t_replicas[0], s.undeliveredPackets, s.constants.config.replica_ids[0])
+  )
+  && (forall pkt :: pkt in s.undeliveredPackets && pkt.msg.v.RslMessage_1b?
+  ==> pkt.src in s.constants.config.replica_ids[0..]
+  )
+  && Phase1GenericInvariant(s)
+}
+
+predicate Phase2Invariant(s:TimestampedRslState)
+  requires RslConsistency(s)
+{
+  && (0 < |s.t_replicas| ==>
+    && s.t_replicas[0].v.replica.proposer.current_state == 2
   )
 }
 
@@ -158,15 +245,9 @@ lemma lemma_RslInitImpliesInitInv(s:TimestampedRslState)
 {
 }
 
-function MultisetToSet<S(!new)>(m:multiset<S>) : set<S>
-  ensures forall x :: x in m <==> x in MultisetToSet(m)
-{
-  set x | x in m :: x
-}
-
-lemma lemma_0_1_InitGoesToPhase1(s:TimestampedRslState, s':TimestampedRslState, j:int)
+lemma lemma_0_1_InitGoesToPhase1NoLeader1b(s:TimestampedRslState, s':TimestampedRslState, j:int) returns (leader_1a_pkt:TimestampedRslPacket)
   requires RslAssumption(s);
-  requires ViewAlwaysZero(s)
+  requires RslAssumption(s');
   requires RslConsistency(s);
   requires RslConsistency(s');
   requires 0 == j < |s.constants.config.replica_ids|
@@ -178,50 +259,60 @@ lemma lemma_0_1_InitGoesToPhase1(s:TimestampedRslState, s':TimestampedRslState, 
   requires TimestampedRslNextOneReplica(s, s', j, s.t_environment.nextStep.ios);
 
   requires InitInvariant(s)
-  ensures Phase1Invariant(s')
+  ensures Phase1UnpreparedLeaderInvariant(s', leader_1a_pkt)
 {
-  // var ios := s.t_environment.nextStep.ios;
-  // var newPacketsSeq := ExtractSentPacketsFromIos(ios);
-  // var newPackets := set x | (x in s'.undeliveredPackets && x !in s.undeliveredPackets) :: x;
-
-  // assume (MultisetToSet(s'.undeliveredPackets) - MultisetToSet(s.undeliveredPackets)) <= (set io | io in ios && io.LIoOpSend? :: io.s);
-  // assume newPackets <= (set io | io in ios && io.LIoOpSend? :: io.s);
-  // assume forall pkt :: (pkt in s'.undeliveredPackets && pkt !in s.undeliveredPackets) ==> ;
-  // assert forall pkt :: pkt in newPackets ==> pkt.msg.v.RslMessage_1a?;
-  // D := (A - B) + C
-  // (D - A) <= C
-
+  var t_ios := s.t_environment.nextStep.ios;
+  var ios := UntagLIoOpSeq(t_ios);
+  var sent_packets := ExtractSentPacketsFromIos(ios);
+  assert LIoOpSend(sent_packets[0]) in ios;
+  var i :| 0 <= i < |ios| && ios[i] == LIoOpSend(sent_packets[0]);
+  leader_1a_pkt := t_ios[i].s;
 }
 
-lemma lemma_InitGoesToInitOrPhase1(s:TimestampedRslState, s':TimestampedRslState, j:int)
+lemma lemma_InitGoesToInitOrPhase1NoLeader1b(s:TimestampedRslState, s':TimestampedRslState, j:int)
   requires RslAssumption(s);
-  requires ViewAlwaysZero(s)
+  requires RslAssumption(s');
   requires RslConsistency(s);
   requires RslConsistency(s');
-  requires 0 <= j < |s.constants.config.replica_ids|
+  requires 0 <= j < |s.constants.config.replica_ids|;
 
   requires s.t_environment.nextStep.LEnvStepHostIos?;
+  requires !(j == 0 && s.t_environment.nextStep.nodeStep == RslStep(1));
   requires s.t_environment.nextStep.actor == s.constants.config.replica_ids[j];
 
   requires TimestampedRslNextOneReplica(s, s', j, s.t_environment.nextStep.ios);
 
   requires InitInvariant(s)
-  ensures InitInvariant(s') || Phase1Invariant(s')
+  ensures InitInvariant(s')
 {
-  if (s.t_replicas[0].v.nextActionIndex == 1) {
-    if (j == 0) {
-        assert Phase1Invariant(s');
-    } else {
-        assert InitInvariant(s');
-    }
-  } else {
-    assert InitInvariant(s');
-  }
 }
 
-lemma lemma_0_j_Phase1GoesToPhase1(s:TimestampedRslState, s':TimestampedRslState, j:int)
+lemma lemma_notleader_nonetwork_Phase1UnpreparedLeaderGoesToPhase1UnpreparedLeader(s_prev:TimestampedRslState, s:TimestampedRslState, j:int, pkt:TimestampedRslPacket)
+  requires RslAssumption(s_prev);
   requires RslAssumption(s);
-  requires ViewAlwaysZero(s)
+  requires RslConsistency(s_prev);
+  requires RslConsistency(s);
+  requires 0 <= j < |s_prev.constants.config.replica_ids|
+
+  requires j > 0;
+
+  requires s_prev.t_environment.nextStep.LEnvStepHostIos?;
+  requires s_prev.t_environment.nextStep.actor == s_prev.constants.config.replica_ids[j];
+  requires s_prev.t_environment.nextStep.nodeStep != RslStep(0)
+  // requires s_prev.t_environment.nextStep.nodeStep != RslStep(2)
+  // requires s_prev.t_environment.nextStep.nodeStep == RslStep(3)
+
+  requires TimestampedRslNextOneReplica(s_prev, s, j, s_prev.t_environment.nextStep.ios);
+
+  requires Phase1UnpreparedLeaderInvariant(s_prev, pkt);
+  ensures Phase1UnpreparedLeaderInvariant(s, pkt);
+{
+  assert ReplicasDistinct(s_prev.constants.config.replica_ids, 0, j);
+}
+
+lemma lemma_notleader_0_Phase1UnpreparedLeaderGoesToPhase1UnpreparedLeader(s:TimestampedRslState, s':TimestampedRslState, j:int, pkt:TimestampedRslPacket)
+  requires RslAssumption(s);
+  requires RslAssumption(s');
   requires RslConsistency(s);
   requires RslConsistency(s');
   requires 0 <= j < |s.constants.config.replica_ids|
@@ -234,20 +325,56 @@ lemma lemma_0_j_Phase1GoesToPhase1(s:TimestampedRslState, s':TimestampedRslState
 
   requires TimestampedRslNextOneReplica(s, s', j, s.t_environment.nextStep.ios);
 
-  requires Phase1Invariant(s)
-  ensures Phase1Invariant(s')
+  requires Phase1UnpreparedLeaderInvariant(s, pkt);
+  ensures Phase1UnpreparedLeaderInvariant(s', pkt);
 {
-  assert ReplicasDistinct(s.constants.config.replica_ids, 0, j);
   var ios := s.t_environment.nextStep.ios;
+  assert ReplicasDistinct(s.constants.config.replica_ids, 0, j);
   if ios[0].LIoOpReceive? {
-    // assert s.t_replicas[j].v.replica.acceptor.max_bal == Ballot(0, 0);
     assert ios[0].r.msg.v.RslMessage_1a?;
-    BoundedLagImpliesBoundedProcessingTime(s.t_replicas[j].dts, s.t_replicas[j].ts, ios[0].r.msg.ts, s'.t_replicas[j].ts);
-  } else {
-    assert Phase1Invariant(s');
+    assert ios[0].r.src == s.constants.config.replica_ids[0];
+    BoundedLagImpliesBoundedProcessingTime(s.t_replicas[j].dts, s.t_replicas[j].ts, ios[0].r.msg.ts, s'.t_replicas[j].ts, TimeActionRange(0));
   }
 }
 
+lemma lemma_leader_0_Phase1UnpreparedLeaderGoesToPhase1(s:TimestampedRslState, s':TimestampedRslState, j:int, pkt:TimestampedRslPacket)
+  requires RslAssumption(s);
+  requires RslAssumption(s');
+  requires RslConsistency(s);
+  requires RslConsistency(s');
+  requires 0 <= j < |s.constants.config.replica_ids|
+
+  requires j == 0
+
+  requires s.t_environment.nextStep.LEnvStepHostIos?;
+  requires s.t_environment.nextStep.actor == s.constants.config.replica_ids[j];
+  requires s.t_environment.nextStep.nodeStep == RslStep(0)
+
+  requires TimestampedRslNextOneReplica(s, s', j, s.t_environment.nextStep.ios);
+
+  requires Phase1UnpreparedLeaderInvariant(s, pkt)
+  ensures Phase1UnpreparedLeaderInvariant(s', pkt) || Phase1PreparedLeaderInvariant(s')
+{
+  reveal_PacketDeliveredInOrder();
+  var ios := s.t_environment.nextStep.ios;
+  if ios[0].LIoOpReceive? {
+    // assert s.t_replicas[j].v.replica.acceptor.max_bal == Ballot(0, 0);
+    if ios[0].r.msg.v.RslMessage_1b? {
+      assert ios[0].r.msg.ts <= pkt.msg.ts;
+      assert pkt.msg.ts <= TimeBound1aSelfDelivery();
+      assert TimeBound1aSelfDelivery() < ios[0].r.msg.ts;
+      assert false;
+    }
+    assert ios[0].r == pkt;
+    assert ios[0].r.src == s.constants.config.replica_ids[0];
+    BoundedLagImpliesBoundedProcessingTime(s.t_replicas[j].dts, s.t_replicas[j].ts, ios[0].r.msg.ts, s'.t_replicas[j].ts, TimeActionRange(0));
+    assert Phase1PreparedLeaderInvariant(s');
+  } else {
+    assert Phase1UnpreparedLeaderInvariant(s', pkt);
+  }
+}
+
+/*
 lemma lemma_a_j_Phase1GoesToPhase1(s:TimestampedRslState, s':TimestampedRslState, j:int)
   requires RslAssumption(s);
   requires ViewAlwaysZero(s)
@@ -268,5 +395,106 @@ lemma lemma_a_j_Phase1GoesToPhase1(s:TimestampedRslState, s':TimestampedRslState
 {
   assert ReplicasDistinct(s.constants.config.replica_ids, 0, j);
 }
+
+lemma lemma_0_0_Phase1GoesToPhase1(s:TimestampedRslState, s':TimestampedRslState, j:int)
+  requires RslAssumption(s);
+  requires RslAssumption(s');
+  requires RslConsistency(s);
+  requires RslConsistency(s');
+  requires 0 <= j < |s.constants.config.replica_ids|
+
+  requires j == 0;
+
+  requires s.t_environment.nextStep.LEnvStepHostIos?;
+  requires s.t_environment.nextStep.actor == s.constants.config.replica_ids[j];
+  requires || s.t_environment.nextStep.nodeStep == RslStep(0);
+
+  requires TimestampedRslNextOneReplica(s, s', j, s.t_environment.nextStep.ios);
+
+  requires Phase1Invariant(s)
+  ensures Phase1Invariant(s')
+{
+  assert forall idx :: 0 < idx < |s'.t_replicas| ==> ReplicasDistinct(s.constants.config.replica_ids, 0, idx);
+  if (s.t_environment.nextStep.nodeStep == RslStep(0)) {
+    var ios := s.t_environment.nextStep.ios;
+    if (ios[0].LIoOpReceive?) {
+      if ios[0].r.msg.v.RslMessage_1b? {
+        var size := |s.t_replicas[0].v.replica.proposer.received_1b_packets|;
+        var size' := |s'.t_replicas[0].v.replica.proposer.received_1b_packets|;
+        assert UntagLPacket(ios[0].r) !in s.t_replicas[0].v.replica.proposer.received_1b_packets;
+        assert s'.t_replicas[0].v.replica.proposer.received_1b_packets == s.t_replicas[0].v.replica.proposer.received_1b_packets + {UntagLPacket(ios[0].r)};
+        assert size' == size + 1;
+        BoundedSizeLagImpliesBoundedProcessingTime(s.t_replicas[j].dts, s.t_replicas[j].ts, ios[0].r.msg.ts, s'.t_replicas[j].ts, size);
+      } else if (ios[0].r.msg.v.RslMessage_1a?) {
+      } else{
+      }
+    } else {
+    }
+  } else if (s.t_environment.nextStep.nodeStep == RslStep(1)) {
+  } else if (s.t_environment.nextStep.nodeStep == RslStep(2)) {
+  } else if (s.t_environment.nextStep.nodeStep == RslStep(3)) {
+  } else if (s.t_environment.nextStep.nodeStep == RslStep(4)) {
+  } else if (s.t_environment.nextStep.nodeStep == RslStep(5)) {
+  } else if (s.t_environment.nextStep.nodeStep == RslStep(6)) {
+  } else if (s.t_environment.nextStep.nodeStep == RslStep(7)) {
+  } else if (s.t_environment.nextStep.nodeStep == RslStep(8)) {
+  } else if (s.t_environment.nextStep.nodeStep == RslStep(9)) {
+  }
+}
+
+lemma lemma_a_0_Phase1GoesToPhase1(s:TimestampedRslState, s':TimestampedRslState, j:int)
+  requires RslAssumption(s);
+  requires RslAssumption(s');
+  requires RslConsistency(s);
+  requires RslConsistency(s');
+  requires 0 <= j < |s.constants.config.replica_ids|
+
+  requires j == 0;
+
+  requires s.t_environment.nextStep.LEnvStepHostIos?;
+  requires s.t_environment.nextStep.actor == s.constants.config.replica_ids[j];
+  requires || s.t_environment.nextStep.nodeStep != RslStep(2);
+  requires || s.t_environment.nextStep.nodeStep != RslStep(0);
+
+  requires TimestampedRslNextOneReplica(s, s', j, s.t_environment.nextStep.ios);
+
+  requires Phase1Invariant(s)
+  ensures Phase1Invariant(s')
+{
+  assert forall idx :: 0 < idx < |s'.t_replicas| ==> ReplicasDistinct(s.constants.config.replica_ids, 0, idx);
+  if (s.t_environment.nextStep.nodeStep == RslStep(0)) {
+  } else if (s.t_environment.nextStep.nodeStep == RslStep(1)) {
+  } else if (s.t_environment.nextStep.nodeStep == RslStep(2)) {
+  } else if (s.t_environment.nextStep.nodeStep == RslStep(3)) {
+  } else if (s.t_environment.nextStep.nodeStep == RslStep(4)) {
+  } else if (s.t_environment.nextStep.nodeStep == RslStep(5)) {
+  } else if (s.t_environment.nextStep.nodeStep == RslStep(6)) {
+  } else if (s.t_environment.nextStep.nodeStep == RslStep(7)) {
+  } else if (s.t_environment.nextStep.nodeStep == RslStep(8)) {
+  } else if (s.t_environment.nextStep.nodeStep == RslStep(9)) {
+  }
+}
+
+lemma lemma_0_0_Phase1GoesToPhase1OrPhase2(s:TimestampedRslState, s':TimestampedRslState, j:int)
+  requires RslAssumption(s);
+  requires RslAssumption(s');
+  requires RslConsistency(s);
+  requires RslConsistency(s');
+  requires 0 <= j < |s.constants.config.replica_ids|
+
+  requires j == 0;
+
+  requires s.t_environment.nextStep.LEnvStepHostIos?;
+  requires s.t_environment.nextStep.actor == s.constants.config.replica_ids[j];
+  requires s.t_environment.nextStep.nodeStep == RslStep(2);
+
+  requires TimestampedRslNextOneReplica(s, s', j, s.t_environment.nextStep.ios);
+
+  requires Phase1Invariant(s)
+  ensures Phase1Invariant(s') // || Phase1Invariant(s')
+{
+}
+
+*/
 
 }
